add spec file

VST-introduction/ASI_kalloc.v
@@ -5,11 +5,9 @@ Require Import VC.helper.
 Global Open Scope funspec_scope.
 
 Record KallocTokenAPD := {
-  kalloc_token': share -> Z -> val -> type -> mpred;
-  kalloc_token'_valid_pointer: forall sh sz p t, 
-  0 < sizeof t ->
-  readable_share sh ->
-      kalloc_token' sh sz p t |-- valid_pointer p;
+  kalloc_token': share -> Z -> val -> mpred;
+  kalloc_token'_valid_pointer: forall sh sz p, 
+  kalloc_token' sh sz p |-- valid_pointer p;
   kalloc_token'_local_facts:  forall sh sz p, 
       kalloc_token' sh sz p |-- !! malloc_compatible sz p;
 }.
@@ -20,7 +18,6 @@ Record KallocFreeAPD := {
 }.
 
 #[export] Hint Resolve kalloc_token'_valid_pointer : valid_pointer. 
-
 #[export] Hint Resolve kalloc_token'_local_facts : saturate_local.
 
 Section Kalloc_ASI.
@@ -28,9 +25,9 @@ Variable K: KallocFreeAPD.
 Variable kalloc1ID: ident.
 Variable kfree1ID: ident.
 
-Definition kfree1_spec := 
+Definition kfree1_spec_sz := 
   DECLARE kfree1ID
-      WITH t:type, new_head:val, gv:globals, sh:share, ls: list val, xx:Z, original_freelist_pointer:val
+      WITH n:Z, new_head:val, gv:globals, sh:share, ls: list val, xx:Z, original_freelist_pointer:val
       PRE [ tptr tvoid]
         PROP(
               is_pointer_or_null new_head
@@ -39,7 +36,7 @@ Definition kfree1_spec :=
         SEP (
           mem_mgr K gv sh ls xx original_freelist_pointer;
           if eq_dec new_head nullval then emp
-          else (kalloc_token' K Ews (sizeof t) new_head t (** data_at_ Ews t new_head*))
+          else (kalloc_token' K sh (n) new_head (* memory_block Ews n new_head*))
         )
       POST [ tvoid ]
         PROP()
@@ -52,13 +49,11 @@ Definition kfree1_spec :=
             ).
 
 
-Definition kalloc1_spec :=
+Definition kalloc1_spec_sz :=
 DECLARE kalloc1ID
-WITH t:type, gv:globals, sh:share, ls: list val, xx:Z, original_freelist_pointer:val
+WITH n:Z, gv:globals, sh:share, ls: list val, xx:Z, original_freelist_pointer:val
 PRE [ ]
-    PROP(0 <= sizeof t <= PGSIZE;
-    complete_legal_cosu_type t = true;
-    natural_aligned natural_alignment t = true) 
+    PROP(0 <= n <= PGSIZE) 
     PARAMS () GLOBALS(gv)
     SEP ( mem_mgr K gv sh ls xx original_freelist_pointer )  
 POST [ tptr tvoid ]
@@ -71,12 +66,14 @@ POST [ tptr tvoid ]
         (
           EX next ls',
           (!! (next :: ls' = ls) &&
-              kalloc_token' K Ews (sizeof t) original_freelist_pointer t *
+              kalloc_token' K sh n original_freelist_pointer *
               mem_mgr K gv sh ls' xx next
         )
         )
     ).
 
-Definition Kalloc_ASI:funspecs := [kalloc1_spec; kfree1_spec].
+Definition Kalloc_ASI:funspecs := [kalloc1_spec_sz; kfree1_spec_sz].
+
 End Kalloc_ASI.
-        
+
+
