VST-introduction/VSU_kalloc_kfree_definitions.v
@@ -9,42 +9,85 @@ Require Import malloc_sep.*)
 
 
 (** token -- could be moved to another file *)
+(*** kalloc token size... *)
+(***** kalloc token size ******)
+Definition kalloc_token_sz (sh: share) (n: Z) (p: val) : mpred :=
+  !! ((*field_compatible t_run [] p /\*)
+      0 < n <= PGSIZE
+      /\ malloc_compatible (n) p 
+      /\ malloc_compatible (PGSIZE) p
+      /\ writable_share sh
+      (*/\  maybe some alignment and physical address checks here *))
+  && memory_block sh (n) (p).
 
-Definition my_kalloc_token (sh: share) (sz: Z) (p: val) (t:type) : mpred := (* my kalloc token is a block where we can have t_run struct in it, but also something else?*)
-  EX v,
-    !! (
-        field_compatible t [] p 
-        /\ malloc_compatible sz p
-        /\ 0 <= sizeof t <= sz
-        /\ writable_share sh) 
-  && (((*memory_block sh (sz) (p *) (data_at sh t v p))). (* this is the rest of the page*)
-  
-
-(** **** Exercise: 2 stars, standard (malloc_token_properties) *)
-Lemma my_kalloc_token_valid_pointer:
-    forall (sh : share) (sz : Z) (p : val) (t: type),
-    0 < sizeof t ->
-    readable_share sh ->
-      my_kalloc_token sh sz p t |-- valid_pointer p.
-Proof.
-  intros.
-  unfold my_kalloc_token. entailer!.
-  apply data_at_valid_ptr; try rep_lia; auto.
-Qed.
-
-Lemma  my_kalloc_token_local_facts : 
-   forall (sh : share) (sz : Z) (p : val) (t:type),
-     my_kalloc_token sh sz p t |-- !! malloc_compatible sz p.
+Lemma kalloc_token_sz_valid_pointer:
+  forall (sh : share) (sz : Z) (p : val),
+  kalloc_token_sz sh sz p |-- valid_pointer p.
 Proof.
   intros. 
-  unfold my_kalloc_token. simpl. entailer.
+  unfold kalloc_token_sz. entailer.
 Qed.
 
-(** token -- could be moved to another file *)
+Lemma  kalloc_token_sz_local_facts : 
+ forall (sh : share) (n:Z) (p : val) ,
+   kalloc_token_sz sh n p |-- !! malloc_compatible n p.
+Proof.
+  intros. 
+  unfold kalloc_token_sz. simpl. entailer.
+Qed.
+
+(******************************)
+
+(*** kalloc token type... *)
+Definition my_kalloc_token {cs: compspecs} sh t p :=
+  !! field_compatible t [] p && (* this shoudl work because of memory_block_data_at_*)
+  (kalloc_token_sz sh (sizeof t) p).
+
+Lemma my_kalloc_token_valid_pointer:
+  forall (sh : share) (t : type) (p : val),
+  my_kalloc_token sh t p |-- valid_pointer p.
+Proof.
+  intros. 
+  unfold my_kalloc_token. unfold kalloc_token_sz. entailer!.
+Qed.
+
+Ltac kalloc_token_data_at_valid_pointer :=
+  match goal with |- ?A |-- valid_pointer ?p =>
+   match A with
+   | context [my_kalloc_token _ _ ?t p] =>
+         try (assert (sizeof t <= 0)
+	  by (simpl sizeof in *; rep_lia); fail 1);
+         try (assert (sizeof t > 0)
+	  by (simpl sizeof in *; rep_lia); fail 1);
+         destruct (zlt 0 (sizeof t));
+         auto with valid_pointer
+   | context [kalloc_token_sz _ _ ?n p] =>
+         try (assert (n <= 0) by rep_lia; fail 1);
+         try (assert (n > 0) by rep_lia; fail 1);
+         destruct (zlt 0 n);
+         auto with valid_pointer
+   end
+ end.
+
+#[export] Hint Extern 1 (my_kalloc_token _ _ _ _ |-- valid_pointer _) =>
+  (simple apply my_kalloc_token_valid_pointer; data_at_valid_aux) : valid_pointer.
+#[export] Hint Extern 4 (_ |-- valid_pointer _) => kalloc_token_data_at_valid_pointer : valid_pointer.
+
+Lemma my_kalloc_token_local_facts:  forall {cs: compspecs} sh t p,
+      my_kalloc_token sh t p |-- !! (field_compatible t [] p /\ malloc_compatible (sizeof t) p).
+Proof. intros.
+ unfold my_kalloc_token.
+ normalize. rewrite prop_and.
+ apply andp_right. apply prop_right; auto.
+ apply kalloc_token_sz_local_facts.
+Qed.
+#[export] Hint Resolve my_kalloc_token_local_facts : saturate_local.
 
 
-Definition Tok_APD := Build_KallocTokenAPD my_kalloc_token my_kalloc_token_valid_pointer
-   my_kalloc_token_local_facts.
+
+Definition Tok_APD := Build_KallocTokenAPD kalloc_token_sz kalloc_token_sz_valid_pointer
+  kalloc_token_sz_local_facts.
+
 
 Definition mem_mgr (gv: globals) (sh : share) (ls: list val) (xx:Z) (original_freelist_pointer:val): mpred := (* I am unsure how to access all these elements.. *)
     !! (writable_share sh /\
@@ -55,7 +98,7 @@ Definition mem_mgr (gv: globals) (sh : share) (ls: list val) (xx:Z) (original_fr
       (sepcon (data_at sh t_struct_kmem (Vint (Int.repr xx), original_freelist_pointer) (gv _kmem))
       (freelistrep sh ls original_freelist_pointer)).
 
-(************ mem_mgr lemmas etc. *************)
+(************ lemmas etc. *************)
 Lemma mem_mgr_split: 
  forall (gv:globals) (sh:share) (ls: list val) (xx:Z) (original_freelist_pointer:val),
   mem_mgr gv sh ls xx original_freelist_pointer
@@ -73,27 +116,35 @@ Proof.
   - unfold mem_mgr. entailer!.
 Qed.
 
-
-Lemma kalloc_token'_split: 
- forall  (sh: share) (sz: Z) (p: val) (t:type),
- my_kalloc_token  (sh) (sz) (p) (t)
-  = 
-  EX v,
-    !! (
-        field_compatible t [] p 
-        /\ malloc_compatible sz p
-        /\ 0 <= sizeof t <= sz
-        /\ writable_share sh) 
-  && (((*memory_block sh (sz) (p *) (data_at sh t v p))).
+Lemma kalloc_token_sz_split:
+forall  (sh: share) (n: Z) (p: val),
+  kalloc_token_sz sh n p =
+  !! ((*field_compatible t_run [] p /\*)
+  0 < n <= PGSIZE
+  /\ malloc_compatible (n) p 
+  /\ malloc_compatible (PGSIZE) p
+  /\ writable_share sh
+  (*/\  maybe some alignment and physical address checks here *))
+  && memory_block sh (n) (p).
 Proof.
   intros. apply pred_ext.
-  - unfold my_kalloc_token. entailer. entailer!. Exists v. entailer!.
-  - unfold my_kalloc_token. entailer!. Exists v. entailer!.
+  - unfold kalloc_token_sz. entailer.
+  - unfold kalloc_token_sz. entailer!.
 Qed.
 
+Lemma my_kalloc_token_split: 
+ forall (sh: share) (t: type) (p: val),
+ my_kalloc_token (sh) (t) (p)
+  = 
+  !! field_compatible t [] p &&
+  (kalloc_token_sz sh (sizeof t) p).
+Proof.
+  intros. apply pred_ext.
+  - unfold my_kalloc_token. entailer.
+  - unfold my_kalloc_token. entailer!.
+Qed.
 
-
-(************ mem_mgr lemmas etc. end *************)
+(************ lemmas etc. end *************)
 
 
 Definition KF_APD := Build_KallocFreeAPD Tok_APD mem_mgr.
