VST-introduction/Spec_kalloc.v
@@ -1,0 +1,86 @@
+(** abstract spec interface *)
+Require Import VST.floyd.proofauto.
+Require Import VC.helper.
+Require Import VC.ASI_kalloc.
+Require Import VC.client1.
+Require Import VC.VSU_kalloc_kfree_definitions.
+
+Global Open Scope funspec_scope.
+
+Definition kfree1_spec (K:KallocFreeAPD) {cs: compspecs} (t: type) := 
+  DECLARE _kfree1
+      WITH new_head:val, gv:globals, sh:share, ls: list val, xx:Z, original_freelist_pointer:val
+      PRE [ tptr tvoid]
+        PROP(
+              is_pointer_or_null new_head
+              ) 
+        PARAMS (new_head) GLOBALS(gv)
+        SEP (
+          ASI_kalloc.mem_mgr K gv sh ls xx original_freelist_pointer;
+          if eq_dec new_head nullval then emp
+          else (my_kalloc_token sh (t) new_head (* data_at_ Ews t new_head*))
+        )
+      POST [ tvoid ]
+        PROP()
+        RETURN () 
+        SEP (
+          if eq_dec new_head nullval then 
+          ASI_kalloc.mem_mgr K gv sh ls xx original_freelist_pointer
+          else 
+          ASI_kalloc.mem_mgr K gv sh (original_freelist_pointer::ls) xx new_head
+            ).
+
+Definition kalloc1_spec (K:KallocFreeAPD) {cs: compspecs} (t: type) :=
+DECLARE _kalloc1
+WITH n:Z, gv:globals, sh:share, ls: list val, xx:Z, original_freelist_pointer:val
+PRE [ ]
+    PROP(0 <= n <= PGSIZE;
+            complete_legal_cosu_type t = true;
+            natural_aligned natural_alignment t = true) 
+    PARAMS () GLOBALS(gv)
+    SEP ( ASI_kalloc.mem_mgr K gv sh ls xx original_freelist_pointer )  
+POST [ tptr tvoid ]
+    PROP()
+    RETURN (original_freelist_pointer) 
+    SEP (
+      if (eq_dec original_freelist_pointer nullval) then
+      ASI_kalloc.mem_mgr K gv sh ls xx original_freelist_pointer * emp
+      else 
+        (
+          EX next ls',
+          (!! (next :: ls' = ls) &&
+              my_kalloc_token sh t original_freelist_pointer *
+              ASI_kalloc.mem_mgr K gv sh ls' xx next
+        )
+        )
+    ).
+
+  Lemma kalloc1_spec_sub:
+    forall  (K:KallocFreeAPD) {cs: compspecs} (t: type), 
+      funspec_sub (snd (kalloc1_spec_sz K _kalloc1)) (snd (kalloc1_spec K t)).
+   Proof.
+     do_funspec_sub. 
+      entailer.
+      Exists w emp. entailer.
+      repeat destruct w.
+      repeat destruct p.
+      entailer.
+      entailer!. intros. destruct (EqDec_val (eval_id ret_temp x) nullval).
+      entailer!.
+      Intros next ls'. Exists next ls'.
+      entailer!.
+      admit.
+Admitted.
+
+Lemma kfree1_spec_sub:
+forall  (K:KallocFreeAPD) {cs: compspecs} (t: type), (* TODO: fix: this is not general, but it uses KF_APD *)
+  funspec_sub (snd (kfree1_spec_sz KF_APD _kfree1)) (snd (kfree1_spec KF_APD t)).
+Proof.
+  do_funspec_sub. 
+  destruct w.
+  repeat (destruct p).
+  Exists (sizeof t, v0, g0, s, l, z, v) emp.
+  entailer!.
+  destruct (EqDec_val v0 nullval) eqn:Heq; entailer.
+  unfold my_kalloc_token. entailer.
+Qed.
