VST-introduction/verif_client_pipe.v
@@ -3,6 +3,7 @@ Require Import VC.ASI_kalloc.
 Require Import VC.client1.
 Require Import VC.helper.
 Require Import VC.VSU_kalloc_kfree_definitions.
+Require Import VC.Spec_kalloc.
 
 
 #[export] Instance CompSpecs : compspecs. make_compspecs prog. Defined.
@@ -39,7 +40,7 @@ Definition client_11_pipealloc_spec : ident * funspec :=
         else
         EX next ls',
           (!! (next :: ls' = ls) &&
-                pipe_rep Ews original_freelist_pointer *
+                pipe_rep sh original_freelist_pointer *
                 MF_globals gv  sh ls' xx next
         )
         )
@@ -54,7 +55,7 @@ Definition client1_spec :=
         SEP (
             MF_globals gv  sh ls xx original_freelist_pointer *
             (if eq_dec new_head nullval then emp
-            else (kalloc_token' KF_APD Ews (sizeof t_run) new_head t_run))
+            else (kalloc_token' KF_APD sh (sizeof t_run) new_head))
         )
     POST [ tptr tvoid ]
         EX r,
@@ -74,10 +75,10 @@ Definition client1_spec :=
                     (!! (next :: ls' = ls) &&
                         MF_globals gv  sh ls' xx next
                     ) *  
-                    kalloc_token' KF_APD Ews (sizeof t_run) original_freelist_pointer t_run)))
+                    kalloc_token' KF_APD sh (sizeof t_run) original_freelist_pointer)))
             else (
                 MF_globals gv  sh ls xx original_freelist_pointer* (* is this still wrong?? *)
-                kalloc_token' KF_APD Ews (sizeof t_run) new_head t_run) )
+                kalloc_token' KF_APD sh (sizeof t_run) new_head) )
             ).
 
                             
@@ -87,7 +88,8 @@ Lemma body_client_11_pipealloc: semax_body MFVprog MFGprog f_client_11_pipealloc
 Proof.
 start_function.
 forward.
-forward_call (t_struct_pipe, gv,  sh,  ls , xx,  original_freelist_pointer).  (* kalloc *)
+forward_call (kalloc1_spec_sub KF_APD t_struct_pipe) (sizeof t_struct_pipe, gv, sh , ls, xx, original_freelist_pointer ). (* kalloc *)
+(*forward_call ((sizeof t_struct_pipe), gv,  sh,  ls , xx,  original_freelist_pointer).*)
 - unfold MF_globals. entailer!. 
 - destruct (eq_dec original_freelist_pointer nullval) eqn:e0.
     + forward_if.
@@ -95,37 +97,42 @@ forward_call (t_struct_pipe, gv,  sh,  ls , xx,  original_freelist_pointer).  (*
         * forward. entailer.
     + Intros ab. forward_if.
         *
-        rewrite mem_mgr_split. entailer. 
-        assert(isptr original_freelist_pointer). {
-        destruct original_freelist_pointer; auto_contradict.
-        - unfold is_pointer_or_null in PNoriginal_freelist_pointer. simpl in PNoriginal_freelist_pointer.
-        subst. auto_contradict.
-        - auto.
-        }
-        destruct original_freelist_pointer; auto_contradict. admit.
-        * rewrite kalloc_token'_split. Intros v. forward. forward. forward. forward. Exists (fst ab) (snd ab).
+        rewrite mem_mgr_split. rewrite my_kalloc_token_split. Intros. rewrite kalloc_token_sz_split.
+        Intros. entailer!.
+        *
+        rewrite mem_mgr_split. rewrite my_kalloc_token_split. Intros. rewrite kalloc_token_sz_split.
+        Intros. 
+        rewrite memory_block_data_at_; auto. rewrite data_at__eq. Intros. forward.
+        forward. forward. forward. 
         entailer.
-        unfold MF_globals. unfold pipe_rep.  Exists (fst v). entailer!.
+        Exists  (fst ab) (snd ab). entailer.
+        unfold MF_globals. unfold pipe_rep.  Exists (fst (default_val t_struct_pipe)). entailer!.
+        rewrite mem_mgr_split. entailer.
         * forward. entailer.
-Admitted.
+Qed.
 
 Lemma body_client1: semax_body MFVprog MFGprog f_client1 client1_spec.
 Proof.
-start_function. 
-forward_call (t_run, new_head, gv, sh, ls, xx:Z, original_freelist_pointer).  (* kfree *)
+start_function.
+forward_call (kfree1_spec_sub KF_APD t_run) (new_head, gv, sh , ls, xx, original_freelist_pointer).
+(*forward_call (kfree1_spec_sub t_run) (sizeof t_struct_pipe, gv, sh , ls, xx, original_freelist_pointer ). (* kalloc *)*)
+
+(*forward_call (t_run, new_head, gv, sh, ls, xx:Z, original_freelist_pointer).  (* kfree *)*)
     + destruct (eq_dec new_head nullval).
         *unfold MF_globals. entailer!.
-        * unfold MF_globals. entailer!. apply derives_refl.
+        * unfold MF_globals. entailer!. admit. (*apply derives_refl.*)
     + destruct (eq_dec new_head nullval).
-        *forward_call (t_run, gv, sh, ls, xx, original_freelist_pointer).  (* kalloc *)
+        *forward_call (kalloc1_spec_sub KF_APD t_run) (sizeof t_run, gv, sh , ls, xx, original_freelist_pointer ). (* kalloc *)
+        (*forward_call (t_run, gv, sh, ls, xx, original_freelist_pointer).  (* kalloc *)*)
         destruct (eq_dec original_freelist_pointer nullval).
             -- forward. Exists nullval. unfold MF_globals. entailer!.
             -- destruct ls.
                 ++ forward. auto_contradict.
                 ++ forward. Exists original_freelist_pointer. entailer. Exists v. entailer.
-                    Exists ls. entailer. unfold MF_globals. entailer!. inversion H0; subst. entailer!.
-        *forward_call (t_run, gv, sh, original_freelist_pointer::ls, xx, new_head).  (* kalloc *)
+                    Exists ls. entailer. unfold MF_globals. entailer!. inversion H0; subst. entailer!. admit. (* should be equal.. *)
+        *forward_call (kalloc1_spec_sub KF_APD t_run) (sizeof t_run,  gv, sh, original_freelist_pointer::ls, xx, new_head ). (* kalloc *)
+        (*forward_call (t_run, gv, sh, original_freelist_pointer::ls, xx, new_head).  (* kalloc *)*)
         destruct (eq_dec new_head nullval).
             -- forward.
             -- forward. Exists new_head. entailer. inversion H0; subst; entailer. unfold MF_globals. entailer!.
-Qed.
+Admitted.
